Added hoare/separation logic

Hoare_Logic.thy
@@ -1,23 +1,201 @@
 theory Hoare_Logic
-imports Translation_Test "algebra/rg-algebra/AbstractAtomicTest/Programming_Constructs"
+  imports Translation_Test "algebra/rg-algebra/AbstractAtomicTest/Programming_Constructs" 
+  "../jormungand/sep_algebra/Sep_Tactics"
 begin
 
 declare [[show_sorts=false]]
 
 
-lemma "((converse (R \<triangleright> P)) `` Q) \<triangleleft> (R \<triangleright> P) = (R \<triangleright> (P \<inter> Q))" nitpick
-  apply (safe; clarsimp simp: restrict_range_def Image_iff restrict_domain_def) 
-
-lemma "(P \<inter> Q\<inverse> `` P') \<triangleleft> Q \<subseteq> (P \<inter> Q\<inverse> `` P') \<triangleleft> Q \<triangleright> P'" nitpick
-
 lemma Id_on_relcomp_eq: "Id_on P O Id_on Q = Id_on (P \<inter> Q)" 
   by (safe; clarsimp simp: Id_on_def, rule relcompI, blast, blast)
+
+
+instantiation option :: (type) stronger_sep_algebra begin
+
+fun sep_disj_option :: "'b option \<Rightarrow> 'b option \<Rightarrow> bool" where
+ "sep_disj_option (Some x) (Some y) = False" | 
+ "sep_disj_option x y = True" 
+
+fun plus_option where
+ "plus_option (Some x) (Some y) = Some x" | 
+ "plus_option (None) y = y" |
+ "plus_option  x (None) = x"
+
+lemma [simp]: "x + None = x"
+  by (case_tac x; clarsimp)
+
+definition "zero_option = None"
+
+instance
+  apply (standard, case_tac x; (clarsimp simp: zero_option_def)?)
+     apply (case_tac x; case_tac y; clarsimp)
+      apply (case_tac x; case_tac y; clarsimp)
+      apply (case_tac x; case_tac y; clarsimp)
+   apply (case_tac x; case_tac y; case_tac z; clarsimp)
+  done
+end
+
+instantiation "fun" :: (type, stronger_sep_algebra) stronger_sep_algebra begin
+
+definition sep_disj_fun :: "('a \<Rightarrow> 'b) \<Rightarrow> ('a \<Rightarrow> 'b) \<Rightarrow> bool" where
+ "sep_disj_fun f g \<equiv> (\<forall>x. f x ## g x)" 
+
+definition plus_fun where
+ "plus_fun f g = (\<lambda>x. f x + g x)"
+
+lemma [simp]: "x + None = x"
+  by (case_tac x; clarsimp)
+
+definition "zero_fun = (\<lambda>x. 0)"
+
+instance
+  apply (standard; (rule ext)?, (clarsimp simp: plus_fun_def sep_disj_fun_def zero_fun_def)? )
+     apply (metis sep_disj_commute)
+  apply (metis sep_add_commute)
+   apply (metis sep_add_assoc)
+  apply (blast)
+  done
+end
+
+instantiation prod :: (stronger_sep_algebra, stronger_sep_algebra) stronger_sep_algebra begin
+
+fun sep_disj_prod :: "'a \<times> 'b \<Rightarrow> 'a \<times> 'b \<Rightarrow> bool" where
+ "sep_disj_prod (a,b) (x,y) \<longleftrightarrow> (a ## x \<and> b ## y)" 
+
+fun plus_prod where
+ "plus_prod (a,b) (x,y) = (a + x, b + y)" 
+
+
+definition "zero_prod = (0,0)"
+
+instance
+  apply (standard, case_tac x; (clarsimp simp: zero_prod_def split: prod.splits)?)
+     apply (metis sep_disj_commute)
+  apply (metis sep_add_commute)
+   apply (metis sep_add_assoc)
+  by blast
+
+end
+
+instantiation unit ::  stronger_sep_algebra begin
+
+fun sep_disj_unit :: "unit \<Rightarrow> unit \<Rightarrow> bool" where
+ "sep_disj_unit x y \<longleftrightarrow> True" 
+
+fun plus_unit :: "unit \<Rightarrow> unit \<Rightarrow> unit" where
+ "plus_unit x y = ()" 
+
+
+definition "zero_unit = ()"
+
+instance
+  by (standard, case_tac x; (clarsimp simp: zero_unit_def)?)
+ 
+
+end
+
+
+
+
+
+instantiation BeaconState_ext :: (stronger_sep_algebra) stronger_sep_algebra begin
+
+
+definition sep_disj_BeaconState_ext :: "'a BeaconState_scheme \<Rightarrow> 'a BeaconState_scheme \<Rightarrow> bool" 
+  where "sep_disj_BeaconState_ext x y == 
+  genesis_time_f x ## genesis_time_f y \<and> 
+  genesis_validators_root_f x ## genesis_validators_root_f y \<and> 
+  slot_f x ## slot_f y \<and> fork_f x ## fork_f y \<and> 
+  latest_block_header_f x ## latest_block_header_f y \<and> 
+  block_roots_f x ##  block_roots_f y \<and>
+  state_roots_f x ##  state_roots_f y \<and> 
+  historical_roots_f x ## historical_roots_f y \<and>
+  eth1_data_f x ## eth1_data_f y \<and>
+  eth1_data_votes_f x ## eth1_data_votes_f y \<and>
+  eth1_deposit_index_f x ## eth1_deposit_index_f y \<and>
+  validators_f x ## validators_f y \<and>
+  balances_f x ## balances_f y \<and>
+  randao_mixes_f x ## randao_mixes_f y \<and>
+  slashings_f x ## slashings_f y \<and>
+  previous_epoch_participation_f x ## previous_epoch_participation_f y \<and>
+  current_epoch_participation_f x ## current_epoch_participation_f y \<and>
+  justification_bits_f x ## justification_bits_f y \<and>
+  previous_justified_checkpoint_f x ## previous_justified_checkpoint_f y \<and>
+  current_justified_checkpoint_f x ## current_justified_checkpoint_f y \<and>
+  finalized_checkpoint_f x ## finalized_checkpoint_f y \<and>
+  inactivity_scores_f x ## inactivity_scores_f y \<and>
+  current_sync_committee_f x ## current_sync_committee_f y \<and>
+  next_sync_committee_f x ## next_sync_committee_f y \<and> BeaconState.more x ## BeaconState.more y"
+
+definition plus_BeaconState_ext :: "'a BeaconState_scheme \<Rightarrow> 'a BeaconState_scheme \<Rightarrow> 'a BeaconState_scheme" 
+  where "plus_BeaconState_ext x y == 
+  \<lparr> genesis_time_f = genesis_time_f x + genesis_time_f y,
+  genesis_validators_root_f = genesis_validators_root_f x + genesis_validators_root_f y, 
+  slot_f = slot_f x + slot_f y, fork_f = fork_f x + fork_f y ,
+  latest_block_header_f = latest_block_header_f x + latest_block_header_f y ,
+  block_roots_f = block_roots_f x + block_roots_f y,
+  state_roots_f = state_roots_f x + state_roots_f y ,
+  historical_roots_f = historical_roots_f x + historical_roots_f y,
+  eth1_data_f = eth1_data_f x + eth1_data_f y,
+  eth1_data_votes_f = eth1_data_votes_f x + eth1_data_votes_f y,
+  eth1_deposit_index_f = eth1_deposit_index_f x + eth1_deposit_index_f y,
+  validators_f = validators_f x + validators_f y,
+  balances_f = balances_f x + balances_f y,
+  randao_mixes_f = randao_mixes_f x + randao_mixes_f y,
+  slashings_f = slashings_f x + slashings_f y,
+  previous_epoch_participation_f = previous_epoch_participation_f x + previous_epoch_participation_f y,
+  current_epoch_participation_f = current_epoch_participation_f x + current_epoch_participation_f y,
+  justification_bits_f = justification_bits_f x + justification_bits_f y,
+  previous_justified_checkpoint_f = previous_justified_checkpoint_f x + previous_justified_checkpoint_f y,
+  current_justified_checkpoint_f = current_justified_checkpoint_f x + current_justified_checkpoint_f y,
+  finalized_checkpoint_f = finalized_checkpoint_f x + finalized_checkpoint_f y,
+  inactivity_scores_f = inactivity_scores_f x + inactivity_scores_f y,
+  current_sync_committee_f = current_sync_committee_f x + current_sync_committee_f y,
+  next_sync_committee_f = next_sync_committee_f x + next_sync_committee_f y, \<dots> = BeaconState.more x + BeaconState.more y \<rparr>"
+
+definition "zero_BeaconState_ext \<equiv> \<lparr> genesis_time_f = None,
+  genesis_validators_root_f = None, 
+  slot_f = None, fork_f = None ,
+  latest_block_header_f = None ,
+  block_roots_f = None,
+  state_roots_f = None ,
+  historical_roots_f = None,
+  eth1_data_f = None,
+  eth1_data_votes_f = None,
+  eth1_deposit_index_f = None,
+  validators_f = None,
+  balances_f = None,
+  randao_mixes_f = None,
+  slashings_f = None,
+  previous_epoch_participation_f = None,
+  current_epoch_participation_f = None,
+  justification_bits_f = None,
+  previous_justified_checkpoint_f = None,
+  current_justified_checkpoint_f = None,
+  finalized_checkpoint_f = None,
+  inactivity_scores_f = None,
+  current_sync_committee_f = None,
+  next_sync_committee_f = None, \<dots> = 0\<rparr>"
+
+instance
+
+  apply (standard; (clarsimp simp: plus_BeaconState_ext_def sep_disj_BeaconState_ext_def zero_BeaconState_ext_def)?)
+     apply (clarsimp simp: sep_disj_commute)
+    apply (metis sep_add_commute)
+   apply (intro conjI; metis sep_add_assoc)
+  apply (safe; clarsimp)
+  done
+end
+
+term "(P \<and>* Q)"
+
+
 
 
 locale hoare_logic = verified_con + strong_spec begin
 
 
-definition "hoare_triple P f Q \<equiv>   run f \<le> assert P; spec (Q) "
+definition "hoare_triple P f Q \<equiv>   run f \<le> assert (Collect P); spec (UNIV \<triangleright> (Collect Q)) "
 
 
 notation hoare_triple ("\<lblot>_\<rblot> _ \<lblot>_\<rblot>")
@@ -31,10 +209,12 @@ lemma setState_spec: "(run (setState s)) \<le> spec (UNIV \<triangleright> {s}) 
     apply (clarsimp simp: run_def setState_def)
   by (meson order_trans spec_ref_pgm spec_term)
 
-lemma set_state_valid: "hoare_triple \<top> (setState s) (UNIV \<triangleright> {s})"
+term eq
+
+lemma set_state_valid: "hoare_triple \<top> (setState s) (eq s)"
   apply (clarsimp simp: hoare_triple_def assert_top)
-  apply (rule setState_spec)
-  done
+  by (metis assert_top seq_nil_left setState_spec top_set_def)
+
 
 lemma getState_spec: "(run (getState)) \<le> spec (UNIV) "
   apply (clarsimp simp: spec_def)
@@ -46,9 +226,10 @@ lemma getState_spec: "(run (getState)) \<le> spec (UNIV) "
 
 lemma getState_valid: "hoare_triple \<top> (getState) \<top>"
   apply (clarsimp simp: hoare_triple_def assert_top)
-  by (simp add: getState_spec spec_test_restricts test_top)
-  apply (rule setState_spec)
-  done
+  apply (simp add: getState_spec spec_test_restricts test_top)
+  by (metis UNIV_eq_I assert_top getState_spec mem_Collect_eq
+            seq_nil_left seq_nil_right test_top top1I)
+
 
 definition "bind_rel P Q = (Id_on P) O Q "
 
@@ -65,9 +246,6 @@ lemma stutter_range_restriction: "a \<in> P \<Longrightarrow> (a,a) \<in> range_
   apply (clarsimp)
   done
 
-lemma stutter_range_restriction: "a \<in> P \<Longrightarrow> (a,a) \<in> Id_on P"
-  apply (clarsimp)
-  done
 
 lemma restrict_domain_compose_Id: "(P \<triangleleft> Q) = ((Id_on P) O Q)" 
   apply (rule set_eqI)
@@ -87,9 +265,6 @@ lemma test_smaller_assert: "p \<subseteq> q \<Longrightarrow> test p ; assert q 
 
 
 
-find_theorems "_ \<triangleright> _ = _"
-lemma "\<lparr>Q\<rparr>; assert P \<le> \<lparr>Q \<triangleright> P\<rparr> ; assert P"
-  find_theorems "spec _ ; assert _"
 
 lemma hoare_chain: "(\<lbrace>P\<rbrace>;\<lparr>Q\<rparr>; \<lbrace>P'\<rbrace>;\<lparr>Q'\<rparr>) \<le> \<lbrace>P - (converse Q `` (-P'))\<rbrace>;\<lparr>(Q) O Q'\<rparr>" 
   apply (subst assert_restricts_spec) back
@@ -117,13 +292,6 @@ lemma univ_sub_neg: "UNIV - P = - P"
   apply (safe; clarsimp)
   done
 
-lemma setState_seq: "hoare_triple P (g ()) Q  \<Longrightarrow>  hoare_triple (- (UNIV \<triangleright> {s})\<inverse> `` (- P)) (do {x <- setState s ; g x}) ( UNIV \<triangleright> {s} O Q) "
-  apply (clarsimp simp: run_def bindCont_def setState_def hoare_triple_def) 
-  apply (rule order_trans)
-   apply (rule seq_mono, rule set_state_hoare_inner, assumption)
-  apply (rule order_trans, subst seq_assoc[symmetric], rule hoare_chain)
-  apply (clarsimp simp: univ_sub_neg)
-  done
 
 lemma setState_seq': "run (g ()) \<le> spec P \<Longrightarrow>  (run (do {x <- setState s ; g x})) \<le> spec (UNIV \<triangleright> {s} O P) "
   apply (clarsimp simp: run_def bindCont_def setState_def)
@@ -148,12 +316,6 @@ lemma pspec_strengthen: "p \<subseteq> q \<Longrightarrow> pspec p \<le> pspec q
 lemma spec_strengthen: "p \<subseteq> q \<Longrightarrow> spec p \<le> spec q" by (erule spec_strengthen)
 
 
-lemma "assert {(a, b)} ; \<lceil>P (a, b)\<rceil> \<le> \<lceil>{(s, s'). (s, s') \<in> P s}\<rceil>"
-  apply (rule order_trans[rotated])
-  thm pspec_strengthen[where p="P (a, b)"]
-   apply (rule pspec_strengthen[where p="P (a, b)"])
-   apply (clarsimp)
-
 lemma restrict_dom_singleton: "restrict_domain {x} {x. P x} = {(a,b). a = x \<and> P (a, b) }"
   apply (clarsimp simp: restrict_domain_def)
   apply (safe)
@@ -169,32 +331,8 @@ lemma test_spec: "test {t} \<le> \<lbrace>UNIV\<rbrace> ; \<lparr>Id_on {t}\<rpa
   apply (clarsimp)
   using test_inf_eq_seq test_seq_commute test_seq_refine by fastforce
 
-lemma "- {(a, b)} \<union> P (a, b) = R"
-  apply (clarsimp simp: Compl_Diff_eq)
 
-  find_theorems uminus "(\<union>)"
-
-lemma getState_seq_gen: "(\<And>x. hoare_triple (P x) (g x) (Q x)) \<Longrightarrow>  hoare_triple (\<Squnion>x. P x \<inter> {x}) (bindCont getState g) ({(s, s'). (s, s') \<in> Q s})"
-  apply (clarsimp simp: run_def bindCont_def getState_def)
-  apply (clarsimp simp: hoare_triple_def run_def Sup_le_iff)
-
-  apply (rule order_trans, rule seq_mono)
-  apply (rule test_spec)
-
-   apply (atomize)
-   apply (erule_tac x="a" in allE)
-   apply (erule_tac x="b" in allE)
-  apply (assumption)
-  apply (rule order_trans, subst seq_assoc[symmetric], rule hoare_chain)
-  apply (clarsimp simp: Diff_eq)
-  apply (rule seq_mono)
-   apply (subst assert_iso[symmetric])
-  apply (rule subsetI)
-   using [[simp_trace]] apply (clarsimp)
-  apply (rule spec_strengthen)
-  apply (clarsimp)
-  done
-  
+named_theorems wp
 
 lemma getState_seq: "(\<And>x. run (g x) \<le> spec (P x)) \<Longrightarrow>  (run (do { x <- getState ; g (x)})) \<le> spec ({(s, s'). (s, s') \<in> P s}) "
   apply (clarsimp simp: run_def bindCont_def getState_def)
@@ -243,18 +381,16 @@ lemma test_prefix_spec: "\<tau> {x} ; spec P \<le> spec {(a, b). a = x \<and> (a
 lemma spec_singletonI[intro!]: "x \<in> S \<Longrightarrow> \<lparr>{x}\<rparr> \<le> \<lparr>S\<rparr>"
   by (simp add: spec_strengthen)
 
-lemma modify_spec: "(run (modifyState f)) \<le> assert UNIV ; spec ({(s, s'). s' = f s})"
-  apply (clarsimp simp: modifyState_def)
-  apply (rule order_trans, rule getState_seq_gen[simplified hoare_triple_def])
-  thm setState_spec
-   apply (rule set_state_valid[simplified hoare_triple_def])
-  apply (clarsimp)
-  apply (clarsimp simp:  assert_top)
-  by (rule spec_strengthen, clarsimp simp: restrict_domain_def restrict_range_def)
 
-lemma hoare_anti_mono: "hoare_triple P' f Q' \<Longrightarrow> P \<subseteq> P' \<Longrightarrow> P \<triangleleft> Q' \<subseteq> Q \<Longrightarrow> hoare_triple P f Q"
+
+lemma hoare_anti_mono: "hoare_triple P' f Q' \<Longrightarrow> P \<le> P' \<Longrightarrow> Q' \<le> Q \<Longrightarrow> hoare_triple P f Q"
   apply (clarsimp simp: hoare_triple_def)
-  by (meson assert_iso dual_order.trans seq_mono_left spec_strengthen_under_pre)
+  apply (rule order_trans)
+   apply (assumption)
+  apply (rule seq_mono)
+  using assert_iso apply blast
+  apply (rule spec_strengthen)
+  by (safe; clarsimp simp: restrict_range_def le_fun_def)
 
 
 lemma restrict_range_UNIV[simp]: "UNIV \<triangleright> S = UNIV \<times> S "
@@ -264,12 +400,6 @@ lemma restrict_range_UNIV[simp]: "UNIV \<triangleright> S = UNIV \<times> S "
 lemma restrict_domain_UNIV[simp]: "UNIV \<triangleleft> R = R "
   by (safe; clarsimp simp: restrict_domain_def) 
 
-lemma modify_spec_valid: "hoare_triple UNIV (modifyState f) {(s, s'). s' = f s}  "
-  apply (clarsimp simp: modifyState_def)
-  apply (rule hoare_anti_mono)
-    apply (rule getState_seq_gen, rule set_state_valid)
-   apply (clarsimp)
-  by (clarsimp)
 
 
 
@@ -291,7 +421,6 @@ lemma if_seq_valid:
   apply (clarsimp split: if_splits)
   done
 
-find_theorems "bindCont _ return"
 
 lemmas if_seq_valid' = if_seq_valid[where c=return, simplified bindCont_return]
 
@@ -301,63 +430,377 @@ lemma run_fail_assert: "run (bindCont fail c) \<le> assert {} ; \<lparr>{}\<rpar
   apply (clarsimp simp: run_def fail_def bindCont_def spec_def pspec_def assert_def)
   using assert_bot local.assert_def by force
 
+lemma Collect_bot[simp]:"Collect \<bottom> = {}"
+  apply (clarsimp)
+  done
 
-lemma run_fail_assert_valid: "hoare_triple {} (bindCont fail c) R"
+lemma run_fail_assert_valid: "hoare_triple \<bottom> (bindCont fail c) R"
   apply (clarsimp simp: run_def fail_def bindCont_def spec_def pspec_def assert_def hoare_triple_def)
   using assert_bot local.assert_def by force
-
-
-lemma assertion_spec: "run (c ()) \<le> assert Q; spec R \<Longrightarrow> run (do {x <- assertion P ; c x}) \<le> assert (Collect P \<inter> Q) ; spec R"
-  apply (clarsimp)
-  apply (clarsimp simp: assertion_def)
-  apply (rule order_trans)
-  apply (subst bindCont_assoc[symmetric])
-   apply (rule getState_seq_gen[simplified hoare_triple_def])
-   apply (rule if_seq)
-    apply (clarsimp simp: bindCont_return', assumption)
-   apply (rule run_fail_assert)
-  apply (rule seq_mono, subst assert_iso[symmetric])
-   apply (clarsimp)
-  apply (rule spec_strengthen, clarsimp split: if_splits)
-  done
 
 declare in_dom_iff[simp]
 
 lemma "x \<in> S \<triangleleft> R \<longleftrightarrow> fst x \<in> S \<and> x \<in> R"
   by (clarsimp simp: restrict_domain_def, safe; clarsimp)
 
-lemma assertion_spec_valid: "hoare_triple Q (c ()) R \<Longrightarrow> hoare_triple (Collect P \<inter> Q) (do {x <- assertion P ; c x}) R"
-  apply (rule hoare_anti_mono)
-  apply (clarsimp simp: assertion_def)
-  apply (subst bindCont_assoc[symmetric])+
-   apply (rule getState_seq_gen)
-   apply (rule if_seq_valid)
-    apply (clarsimp simp: bindCont_return', assumption)
-   apply (rule run_fail_assert_valid[where R="{}"])
-   apply (clarsimp)
-  apply (clarsimp simp:  split: if_splits)
-  done
-
 definition "wf_lens l \<longleftrightarrow> (\<forall>s v. get l (set l s v) = v)"
-
 
 definition "maps_to l v s \<equiv> wf_lens l \<and> get l (fst s) = Some v" 
 
-lemma "hoare_triple (Collect (maps_to l v)) (write_beacon l v') ({(s,s'). maps_to l v s \<and> maps_to l v' s'})"
-  apply (rule hoare_anti_mono)
-    apply (clarsimp simp: write_beacon_def bindCont_assoc[symmetric])
-    apply (rule getState_seq_gen)
-    apply (rule if_seq_valid')
-     apply (rule run_fail_assert_valid[where c=return and R="{}", simplified bindCont_return] )
-    apply (rule set_state_valid)
-   apply (clarsimp simp: maps_to_def)
-  apply (clarsimp split: if_splits)
-  apply (clarsimp simp: maps_to_def )
-  apply (clarsimp simp: wf_lens_def)
+lemma restrict_UNIV_times: "P \<triangleleft> (UNIV \<times> R) = (P \<times> R)"
+  by (safe; clarsimp)
+
+lemma spec_ref_pgm':"R \<subseteq> R' \<Longrightarrow> pgm R \<le> spec R'"
+  by (meson dual_order.trans pgm.hom_mono spec_ref_pgm)
+
+lemma write_beacon_sep: "hoare_triple ( (maps_to l v \<and>* R)) (write_beacon l v') ( (maps_to l v' \<and>* R))"
+  apply (clarsimp simp: hoare_triple_def run_def write_beacon_def bindCont_def getState_def Sup_le_iff)
+  apply (intro conjI impI)
+   apply (clarsimp simp: assert_galois_test)
+   apply (clarsimp simp: seq_assoc[symmetric] test_seq_test)
+   apply (clarsimp simp: fail_def)
+   apply (subgoal_tac "\<tau> (Collect (maps_to l v \<and>* R)) \<sqinter> \<tau> {(a, b)} = \<bottom>"; clarsimp?)
+   defer
+   apply (clarsimp)
+   apply (clarsimp simp: assert_galois_test seq_assoc[symmetric] test_seq_test setState_def pgm_test_pre domain_restrict_twice )
+   apply (clarsimp simp: restrict_UNIV_times)
+   apply (rule spec_ref_pgm')
+   apply (clarsimp)
+  sorry
+
+
+
+
+abbreviation (input) "member S \<equiv> (\<lambda>x. x \<in> S)"
+
+lemma run_read_beacon_split[simp]: "run (bindCont (read l) c) = ((run (read l)) ; (\<Squnion>x. \<tau> {s. get l (fst s) = Some x}  ; run (c x)))"
+  apply (clarsimp simp: run_def bindCont_def read_beacon_def getState_def return_def Nondet_seq_distrib split: if_splits )
+  apply (rule antisym; (clarsimp simp: Sup_le_iff Nondet_seq_distrib)?)
+   apply (safe; (clarsimp split: if_splits)?)
+    apply (rule Sup_upper)
+
+     apply (clarsimp simp: image_iff)
+     apply (rule_tac x=a in exI)
+    apply (rule_tac x=b in exI)
+    apply (safe; clarsimp?)
+    apply (clarsimp simp: fail_def seq_assoc)
+   apply (clarsimp simp: return_def)
+   apply (rule Sup_upper2)
+
+     apply (clarsimp simp: image_iff)
+     apply (rule_tac x=a in exI)
+    apply (rule_tac x=b in exI)
+    apply (safe; clarsimp?)
+  apply (rule refl)
+   apply (clarsimp simp: return_def par.seq_Nondet_distrib)
+   apply (rule Sup_upper2, clarsimp simp: image_iff)
+  apply (rule_tac x=y in exI, rule refl)
+  using seq_mono_left test.hom_mono test_seq_refine apply force
+  apply (safe)
+   apply (clarsimp simp: fail_def)
+ apply (rule Sup_upper2)
+
+     apply (clarsimp simp: image_iff)
+     apply (rule_tac x=a in exI)
+    apply (rule_tac x=b in exI)
+    apply (clarsimp, rule refl, clarsimp simp: fail_def seq_assoc)
+  apply (clarsimp simp: return_def)
+  apply (clarsimp simp: par.seq_Nondet_distrib Sup_le_iff)
+  apply (case_tac "y = aa"; clarsimp?)
+  apply (rule Sup_upper2, clarsimp simp: image_iff)
+
+     apply (rule_tac x=a in exI)
+  apply (rule_tac x=b in exI)
+   apply (clarsimp simp: return_def)
+   apply (rule refl)
+   apply (meson dual_order.refl seq_mono_right test_seq_refine)
+  apply (subst seq_assoc[symmetric], subst test_seq_test)
+  apply (clarsimp)
   done
 
-lemma ifM_seq: "(run (do {x <- ifM B P Q; c x})) \<le> spec R"
-  apply (clarsimp simp: ifM_def bindCont_def run_def)
+
+
+lemma run_write_beacon_split[simp]: "run (bindCont (write_beacon l v') c) = ((run (write_beacon l v')) ; run (c ()))"
+  apply (clarsimp simp: run_def bindCont_def write_beacon_def getState_def)
+  apply (rule antisym; (clarsimp simp: Sup_le_iff Nondet_seq_distrib)?)
+   apply (safe)
+     apply (rule Sup_upper)
+     apply (clarsimp simp: image_iff)
+     apply (rule_tac x=a in exI)
+     apply (rule_tac x=b in exI)
+     apply (safe; clarsimp simp: fail_def)
+     apply (simp add: seq_assoc)
+    apply (rule Sup_upper)
+ apply (clarsimp simp: image_iff)
+     apply (rule_tac x=a in exI)
+     apply (rule_tac x=b in exI)
+     apply (safe; clarsimp simp: fail_def)
+    apply (simp add: seq_assoc)
+    apply (clarsimp simp: setState_def)
+  apply (rule Sup_upper)
+ apply (clarsimp simp: image_iff)
+     apply (rule_tac x=a in exI)
+     apply (rule_tac x=b in exI)
+     apply (safe; clarsimp simp: fail_def)
+   apply (simp add: seq_assoc)
+  apply (rule Sup_upper)
+ apply (clarsimp simp: image_iff)
+     apply (rule_tac x=a in exI)
+     apply (rule_tac x=b in exI)
+     apply (safe; clarsimp simp: fail_def)
+  apply (simp add: seq_assoc)
+  apply (clarsimp simp: setState_def)
+  done
+
+lemma hoare_chain': "Q \<subseteq> P' \<Longrightarrow>
+    (assert P ; spec (UNIV \<times> Q)) ; (assert P' ; spec (UNIV \<times> Q')) \<le> assert P ; spec (UNIV \<times> Q')"
+  apply (subst assert_restricts_spec) back back
+  apply (simp only: restrict_UNIV_times)
+  apply (clarsimp simp: seq_assoc[symmetric])
+  apply (rule order_trans)
+   apply (rule hoare_chain)
+  apply (subst assert_restricts_spec)
+  apply (rule seq_mono)
+   apply (clarsimp simp: assert_iso[symmetric])
+   apply (blast)
+  apply (rule spec_strengthen)
+  apply (clarsimp)
+  done
+
+
+
+lemma write_beacon_wp[wp]: "hoare_triple ( P) (c ()) Q \<Longrightarrow> hoare_triple ( (maps_to l v \<and>* (maps_to l v' \<longrightarrow>* P))) (do {x <- write_beacon l v' ; c x}) ( Q)"
+  apply (clarsimp simp: hoare_triple_def)
+  apply (rule order_trans)
+   apply (rule seq_mono)
+    apply (rule write_beacon_sep[simplified hoare_triple_def, where R="(maps_to l v' \<longrightarrow>* P)"], assumption)
+  apply (clarsimp simp: restrict_range_UNIV)
+  apply (rule hoare_chain', clarsimp)
+  apply (sep_solve)
+  done
+
+
+
+
+lemma read_sep: " hoare_triple ( (maps_to l v \<and>* R)) (read l) ( (maps_to l v \<and>* R))"
+  apply (clarsimp simp: hoare_triple_def run_def read_beacon_def bindCont_def getState_def Sup_le_iff, safe)
+   apply (clarsimp simp: fail_def assert_galois_test)
+   defer
+   apply (clarsimp simp: return_def)
+   apply (metis assert_galois_test nil_ref_test restrict_range_UNIV seq_mono 
+   seq_mono_left seq_nil_left spec_test_restricts spec_univ term_nil test_seq_commute)
+  apply (subgoal_tac "\<tau> (Collect (maps_to l v \<and>* R)) ; \<tau> {(a, b)} \<le> \<bottom>")
+  apply (metis bot.extremum inf.absorb_iff2 inf_bot_left seq_assoc seq_magic_left)
+  sorry
+
+lemma times_restrict_range[simp]: "(UNIV \<times> P) \<triangleright> Q = (UNIV \<times> (P \<inter> Q))"
+  by (safe; (clarsimp simp: restrict_range_def)?)
+
+lemma maps_to_get_wf:"(maps_to l v \<and>* R) (a, b) \<Longrightarrow> get l a = Some v"
+  apply (clarsimp simp: sep_conj_def maps_to_def)
+  sorry
+
+lemma read_beacon_wp[wp]: "hoare_triple ( (P )) (c v) (Q ) \<Longrightarrow> hoare_triple ( (maps_to l v \<and>* (maps_to l v \<longrightarrow>*  (P )))) (do {v <- read_beacon l ; c v}) (Q  )"
+  apply (clarsimp simp: hoare_triple_def bindCont_def run_def read_beacon_def getState_def )
+  apply (clarsimp simp: Sup_le_iff)
+  apply (safe)
+   apply (clarsimp simp: fail_def assert_galois_test)
+   defer
+   apply (clarsimp simp: fail_def assert_galois_test return_def)
+   apply (case_tac "y = v"; clarsimp?)
+    apply (subst seq_assoc[symmetric])
+    apply (subst test_seq_test)
+    apply (rule order_trans, rule seq_mono_left)
+     apply (rule test.hom_mono[where p="Collect (P )"])
+     apply (clarsimp)
+     apply (sep_solve)
+    apply (blast)
+  apply (subst seq_assoc[symmetric])
+   apply (subst test_seq_test)
+ apply (rule order_trans, rule seq_mono_left)
+    apply (rule test.hom_mono[where p="{}"])
+    apply (clarsimp)
+    defer
+    apply (clarsimp)
+  apply (subst seq_assoc[symmetric])
+   apply (subst test_seq_test)
+ apply (rule order_trans, rule seq_mono_left)
+    apply (rule test.hom_mono[where p="{}"])
+    apply (clarsimp)
+    defer
+    apply (clarsimp)
+   apply (drule maps_to_get_wf, clarsimp)
+  apply (drule maps_to_get_wf, clarsimp)
+  done
+ 
+
+definition "swap l l' \<equiv> do {x <- read_beacon l;
+                            y <- read l';
+                            _ <- write_beacon l' x;
+                            write_beacon l  y}"
+
+
+definition "add_fields l l' \<equiv> do {x <- read_beacon l;
+                                  y <- read_beacon l';
+                                  return (x + y)}"
+
+
+definition "set_max a b c \<equiv> do { x <- read_beacon a;
+                                  y <- read_beacon b;
+                                  (if (x \<le> y) then write_beacon c y else write_beacon c x)}"
+
+
+lemma return_wp: "hoare_triple P (return c) P"
+  apply (clarsimp simp: hoare_triple_def)
+  apply (clarsimp simp: run_def return_def)
+  by (metis assert_galois_test restrict_range_UNIV seq_mono_left seq_nil_left seq_nil_right spec_test_restricts spec_univ term_nil)
+
+
+
+
+lemma hoare_strengthen_post: "hoare_triple P f Q' \<Longrightarrow> Q' \<le> Q \<Longrightarrow> hoare_triple P f Q"
+  apply (clarsimp simp: hoare_triple_def le_fun_def)
+  apply (rule order_trans)
+   apply (assumption)
+  apply (rule seq_mono)
+  using assert_iso apply blast
+  apply (rule spec_strengthen)
+  by (fastforce)
+
+lemma hoare_weaken_pre: "hoare_triple P' f Q \<Longrightarrow> P \<le> P' \<Longrightarrow> hoare_triple P f Q"
+  apply (clarsimp simp: hoare_triple_def)
+  apply (rule order_trans)
+   apply (assumption)
+  apply (rule seq_mono)
+  using assert_iso apply blast
+  by (clarsimp)
+
+lemma swap_sep: "hoare_triple ( (maps_to l v \<and>* maps_to l' v' \<and>* R)) (swap l l') ( (maps_to l v' \<and>* maps_to l' v \<and>* R) )"
+  apply (clarsimp simp: swap_def)
+  apply (rule hoare_weaken_pre)
+   apply (rule read_beacon_wp)
+  apply (rule read_beacon_wp[where v=v'])
+   apply (rule wp )+
+  apply (rule  wp[where c=return, simplified bindCont_return, OF return_wp])
+  apply (clarsimp)
+   apply (sep_solve)
+  done
+
+lemma swap_wp: "hoare_triple ( P) (c ()) Q  \<Longrightarrow> hoare_triple ( (maps_to l v \<and>* maps_to l' v' \<and>* (maps_to l v' \<and>* maps_to l' v \<longrightarrow>* P))) (do {x <- swap l l'; c x}) (Q)"
+  apply (clarsimp simp: swap_def)
+  apply (rule hoare_anti_mono)
+    apply (clarsimp simp: bindCont_assoc[symmetric])
+   apply (rule wp )+
+  apply (assumption)
+  apply (clarsimp)
+  apply (sep_cancel)+
+   apply (sep_solve)
+  apply (clarsimp)
+  done
+
+
+lemma return_triple: "hoare_triple P (bindCont C return) Q \<Longrightarrow> hoare_triple P C Q "
+  apply (clarsimp simp: bindCont_return)
+  done
+
+
+method wp = ((simp only: bindCont_assoc[symmetric] bindCont_return')?,
+       (rule wp return_wp wp[THEN return_triple]) | assumption )+ 
+
+lemma add_fields_wp: "(\<And>a. hoare_triple ( (P a)) (c a) (Q))  \<Longrightarrow>
+    hoare_triple ( (maps_to l v \<and>* maps_to l' v' \<and>* (maps_to l v \<and>* maps_to l' v' \<longrightarrow>* P (v + v')))) (do {x <- add_fields l l'; c x}) (Q )"
+  apply (clarsimp simp: add_fields_def)
+  apply (rule hoare_weaken_pre)
+    apply (wp)
+  by (clarsimp, sep_cancel+, sep_solve)
+
+
+thm swap_wp[where c=return, simplified bindCont_return]
+
+thm add_fields_wp[where c=return, simplified bindCont_return]
+
+find_theorems "if _ then _ else _" bindCont
+
+
+ 
+
+
+lemma if_wp[wp]: 
+  "(B \<Longrightarrow> hoare_triple  ( S) ( bindCont P c) R) \<Longrightarrow> (\<not>B \<Longrightarrow> hoare_triple ( S') (bindCont Q c) R) \<Longrightarrow>
+   hoare_triple ( (if B then S else S'))  (do {x <- (if B then P else Q); c x}) R"
+  apply (clarsimp split: if_splits)
+  done
+
+lemma inf_spec: " \<Inter> (range P) \<le> P (a, b)"
+  apply (clarsimp)
+  done
+
+lemma getState_wp[wp]: "(\<And>a. hoare_triple (P a) (c a) Q) \<Longrightarrow> 
+  hoare_triple (\<lambda>x. P x x) (bindCont getState c) Q"
+  apply (clarsimp simp: getState_def hoare_triple_def bindCont_def run_def Sup_le_iff assert_galois_test test_restricts_Nondet)
+  apply (atomize)
+  apply (erule_tac x=a in allE)
+  apply (erule_tac x=b in allE)
+  apply (erule order_trans[rotated])
+  using seq_mono_left test.hom_mono by force
+
+
+lemma run_setState_distrib: "run (bindCont (setState s) c) = run (setState s); run (c ())"
+  by (clarsimp simp: run_def bindCont_def setState_def)
+
+lemma run_setState_le: "run (setState s) \<le> assert UNIV ; spec (UNIV \<times> {s})"
+  apply (clarsimp simp: setState_def run_def)
+  by (simp add: assert_top spec_ref_pgm)
+
+lemma setState_wp[wp]: " hoare_triple (P) (c ()) Q \<Longrightarrow>  
+  hoare_triple (\<lambda>_. P s) (bindCont (setState s) c) Q"
+  apply (clarsimp simp:  hoare_triple_def   Sup_le_iff run_setState_distrib)
+  apply (safe)
+   apply (rule order_trans)
+    apply (rule seq_mono)
+     apply (rule run_setState_le)
+    apply (assumption)
+   apply (rule hoare_chain')
+   apply (blast)
+ apply (rule order_trans)
+    apply (rule seq_mono)
+     apply (rule run_setState_le)
+   apply (assumption)
+  by (simp add: assert_bot)
+  
+
+lemma fail_wp[wp]: "hoare_triple  \<bottom> (bindCont fail c) Q" 
+  using run_fail_assert_valid by force
+
+lemma assert_wp[wp]: 
+  "hoare_triple ( P) (c ()) Q \<Longrightarrow>
+   hoare_triple ( (\<lambda>x. (C x \<longrightarrow> P x) \<and> C x))  (do {x <- (assertion C); c x}) Q"
+  apply (clarsimp split: if_splits)
+  apply (clarsimp simp: assertion_def)
+ 
+  apply (rule hoare_weaken_pre)
+   apply (wp)
+  apply (safe)
+  apply (clarsimp)
+  done
+
+
+
+lemma "hoare_triple ( (maps_to a x \<and>* maps_to b y \<and>* maps_to c z)) (set_max a b c) ( (maps_to a x \<and>* maps_to b y \<and>* maps_to c (max x y)))"
+  apply (clarsimp simp: set_max_def)
+  apply (rule hoare_weaken_pre)
+   apply (wp)
+  apply (safe)
+  apply (sep_cancel)+
+  apply (clarsimp split: if_splits)
+  apply (safe)
+   apply (sep_cancel)+
+   apply (clarsimp simp: max_def)
+   apply (sep_cancel)+
+  apply (clarsimp simp: max_def)
+  done
+ 
+
 
 
 end
