jormungand/Hoare_Sep_Tactics/SP.thy
@@ -1,0 +1,15 @@
+theory SP
+imports
+ Main
+"~~/src/HOL/Eisbach/Eisbach"
+begin
+
+text \<open>Rule collections for strongest postconditions\<close>
+named_theorems sp
+named_theorems sp_pre
+
+text \<open> Strongest postcondition method setup \<close>
+method sp declares sp = ((((rule sp)+), (rule sp_pre, rule sp, assumption?)?)  |
+                        (rule sp_pre, rule sp, assumption?))
+
+end
